CellularAutomatas/proofs/constructions/cart_fix_empty_word.lean
@@ -13,11 +13,11 @@ variable {α: Type} [Alphabet α]
 
 
 def fix_empty (contains_empty: Bool) (C: CA_rt α): CA_rt α :=
-    toRtCa ((C.val.toCellAutomaton ⨂ c_is_border α).map_project (fun (a, b) => if b then contains_empty else a))
+    toRtCa ((C.toCellAutomaton ⨂ c_is_border α).map_project (fun (a, b) => if b then contains_empty else a))
 
 @[simp]
 lemma fix_empty_spec (contains_empty: Bool) (C: CA_rt α)  (w: Word α):
-    w ∈ (fix_empty contains_empty C).val.L ↔ if w == [] then contains_empty else w ∈ C.val.L := by
+    w ∈ (fix_empty contains_empty C).L ↔ if w == [] then contains_empty else w ∈ C.L := by
   rw [CA_rt_L_iff]
   erw [comp_of_map_project]
   rw [ca_zip_comp]
